

Formal Proofs for Rect as a Complete Semidistributive Lattice

Definitions

Let Rect be the set of all axis-aligned rectangles with coordinates $(\text{left}, \text{top}, \text{right}, \text{bottom})$ where $\text{left} \leq \text{right}$ and $\text{top} \leq \text{bottom}$, plus the empty rectangle \emptyset .

Notation Convention

Throughout these proofs, let R_1, R_2, R_3 denote arbitrary rectangles where each is either:

- \emptyset (the empty rectangle), or
- A non-empty rectangle with coordinates, where:
 - $R_n = (l_n, t_n, r_n, b_n)$ with $l_n \leq r_n$ and $t_n \leq b_n$

When specific rectangles are needed, we use $R_1 = (l_1, t_1, r_1, b_1)$, $R_2 = (l_2, t_2, r_2, b_2)$, $R_3 = (l_3, t_3, r_3, b_3)$, etc.

Operations

Join Operation (\mid):

- If $R_1 = \emptyset$, then $R_1 \mid R_2 = R_2$
- If $R_2 = \emptyset$, then $R_1 \mid R_2 = R_1$
- Otherwise: $R_1 \mid R_2 = (\min(l_1, l_2), \min(t_1, t_2), \max(r_1, r_2), \max(b_1, b_2))$

Meet Operation ($\&$):

- If $R_1 = \emptyset$ or $R_2 = \emptyset$, then $R_1 \& R_2 = \emptyset$
- Otherwise: $R_1 \& R_2 = (\max(l_1, l_2), \max(t_1, t_2), \min(r_1, r_2), \min(b_1, b_2))$
 - If the result has $\text{left} > \text{right}$ or $\text{top} > \text{bottom}$, return \emptyset

Identity Elements:

- $\text{EMPTY} = \emptyset$ (the empty rectangle)
- $\text{PLANE} = \square = (-\infty, -\infty, +\infty, +\infty)$ (the infinite plane)

Partial Order: $R_1 \leq R_2$ iff $R_1 \& R_2 = R_1$ (equivalently, $R_1 \mid R_2 = R_2$)

1. Identity Element Proofs

Theorem 1.1: $R_1 \mid \emptyset = R_1$

Proof: By definition of join:

- If $R_1 = \perp$: then $\perp \mid \perp = \perp$ ✓
- If $R_1 \neq \perp$: then $R_1 \mid \perp = R_1$ ✓

■

Theorem 1.2: $R_1 \& \perp = R_1$

Proof: Case 1: $R_1 = \perp$

- By definition, $\perp \& \perp = \perp$ ✓

Case 2: $R_1 \neq \perp$

$$\begin{aligned}
 R_1 \& \perp &= (l_1, t_1, r_1, b_1) \& (-\infty, -\infty, +\infty, +\infty) \\
 &= (\max(l_1, -\infty), \max(t_1, -\infty), \min(r_1, +\infty), \min(b_1, +\infty)) \\
 &= (l_1, t_1, r_1, b_1) \\
 &= R_1 \quad \checkmark
 \end{aligned}$$

■

2. Absorbing Element Proofs

Theorem 2.1: $R_1 \mid \perp = \perp$

Proof: Case 1: $R_1 = \perp$

- $\perp \mid \perp = \perp$ by join definition ✓

Case 2: $R_1 \neq \perp$

$$\begin{aligned}
 R_1 \mid \perp &= (l_1, t_1, r_1, b_1) \mid (-\infty, -\infty, +\infty, +\infty) \\
 &= (\min(l_1, -\infty), \min(t_1, -\infty), \max(r_1, +\infty), \max(b_1, +\infty)) \\
 &= (-\infty, -\infty, +\infty, +\infty) \\
 &= \perp \quad \checkmark
 \end{aligned}$$

■

Theorem 2.2: $R_1 \& \perp = \perp$

Proof: By definition of meet: $R_1 \& \perp = \perp$ ✓

■

3. Idempotency Proofs

Theorem 3.1: $(R_1 \mid R_1 = R_1)$

Proof: Case 1: $(R_1 = \emptyset)$

- $(\emptyset \mid \emptyset = \emptyset)$ by definition ✓

Case 2: $(R_1 \neq \emptyset)$

$$\begin{aligned} R_1 \mid R_1 &= (l_1, t_1, r_1, b_1) \mid (l_1, t_1, r_1, b_1) \\ &= (\min(l_1, l_1), \min(t_1, t_1), \max(r_1, r_1), \max(b_1, b_1)) \\ &= (l_1, t_1, r_1, b_1) \\ &= R_1 \quad \checkmark \end{aligned}$$

■

Theorem 3.2: $(R_1 \& R_1 = R_1)$

Proof: Case 1: $(R_1 = \emptyset)$

- $(\emptyset \& \emptyset = \emptyset)$ by definition ✓

Case 2: $(R_1 \neq \emptyset)$

$$\begin{aligned} R_1 \& R_1 &= (l_1, t_1, r_1, b_1) \& (l_1, t_1, r_1, b_1) \\ &= (\max(l_1, l_1), \max(t_1, t_1), \min(r_1, r_1), \min(b_1, b_1)) \\ &= (l_1, t_1, r_1, b_1) \\ &= R_1 \quad \checkmark \end{aligned}$$

■

4. Commutativity Proofs

Theorem 4.1: $(R_1 \mid R_2 = R_2 \mid R_1)$

Proof: Case 1: Either $(R_1 = \emptyset)$ or $(R_2 = \emptyset)$

- If $(R_1 = \emptyset)$: $(\emptyset \mid R_2 = R_2 = R_2 \mid \emptyset)$ ✓
- If $(R_2 = \emptyset)$: $(R_1 \mid \emptyset = R_1 = \emptyset \mid R_1)$ ✓

Case 2: Both $(R_1 \neq \emptyset)$ and $(R_2 \neq \emptyset)$

$$R_1 \mid R_2 = (\min(l_1, l_2), \min(t_1, t_2), \max(r_1, r_2), \max(b_1, b_2))$$

Since \min and \max are commutative, this equals:

$$(\min(l_2, l_1), \min(t_2, t_1), \max(r_2, r_1), \max(b_2, b_1)) = R_2 \mid R_1 \checkmark$$

■

Theorem 4.2: $R_1 \& R_2 = R_2 \& R_1$

Proof: Case 1: Either $R_1 = \emptyset$ or $R_2 = \emptyset$

- $\emptyset \& R_2 = \emptyset = R_2 \& \emptyset \checkmark$

Case 2: Both $R_1 \neq \emptyset$ and $R_2 \neq \emptyset$

$$R_1 \& R_2 = (\max(l_1, l_2), \max(t_1, t_2), \min(r_1, r_2), \min(b_1, b_2))$$

Since \min and \max are commutative, this equals:

$$(\max(l_2, l_1), \max(t_2, t_1), \min(r_2, r_1), \min(b_2, b_1)) = R_2 \& R_1 \checkmark$$

■

5. Associativity Proofs

Theorem 5.1: $(R_1 \mid R_2) \mid R_3 = R_1 \mid (R_2 \mid R_3)$

Proof: Case 1: Any of R_1 , R_2 , or R_3 is \emptyset

- If $R_1 = \emptyset$: $(\emptyset \mid R_2) \mid R_3 = R_2 \mid R_3 = \emptyset \mid (R_2 \mid R_3) \checkmark$
- If $R_2 = \emptyset$: $(R_1 \mid \emptyset) \mid R_3 = R_1 \mid R_3 = R_1 \mid (\emptyset \mid R_3) \checkmark$
- If $R_3 = \emptyset$: $(R_1 \mid R_2) \mid \emptyset = R_1 \mid R_2 = R_1 \mid (R_2 \mid \emptyset) \checkmark$

Case 2: All non-empty

Left side:

$$R_1 \mid R_2 = (\min(l_1, l_2), \min(t_1, t_2), \max(r_1, r_2), \max(b_1, b_2))$$

$$\begin{aligned} (R_1 \mid R_2) \mid R_3 = & (\min(\min(l_1, l_2), l_3), \\ & \min(\min(t_1, t_2), t_3), \\ & \max(\max(r_1, r_2), r_3), \\ & \max(\max(b_1, b_2), b_3)) \end{aligned}$$

Right side:

$$R_2 \mid R_3 = (\min(l_2, l_3), \min(t_2, t_3), \max(r_2, r_3), \max(b_2, b_3))$$

$$R_1 \mid (R_2 \mid R_3) = (\min(l_1, \min(l_2, l_3)), \\ \min(t_1, \min(t_2, t_3)), \\ \max(r_1, \max(r_2, r_3)), \\ \max(b_1, \max(b_2, b_3)))$$

By associativity of \min and \max , both sides are equal ✓

■

Theorem 5.2: $(R_1 \ \& \ R_2) \ \& \ R_3 = R_1 \ \& \ (R_2 \ \& \ R_3)$

Proof: Case 1: Any of R_1 , R_2 , or R_3 is \varnothing

- $(\varnothing \ \& \ R_2) \ \& \ R_3 = \varnothing \ \& \ R_3 = \varnothing = \varnothing \ \& \ (R_2 \ \& \ R_3)$ ✓
- Similar for $R_2 = \varnothing$ or $R_3 = \varnothing$ ✓

Case 2: All non-empty

Left side:

$$R_1 \ \& \ R_2 = (\max(l_1, l_2), \max(t_1, t_2), \min(r_1, r_2), \min(b_1, b_2))$$

$$(R_1 \ \& \ R_2) \ \& \ R_3 = (\max(\max(l_1, l_2), l_3), \\ \max(\max(t_1, t_2), t_3), \\ \min(\min(r_1, r_2), r_3), \\ \min(\min(b_1, b_2), b_3))$$

Right side:

$$R_2 \ \& \ R_3 = (\max(l_2, l_3), \max(t_2, t_3), \min(r_2, r_3), \min(b_2, b_3))$$

$$R_1 \ \& \ (R_2 \ \& \ R_3) = (\max(l_1, \max(l_2, l_3)), \\ \max(t_1, \max(t_2, t_3)), \\ \min(r_1, \min(r_2, r_3)), \\ \min(b_1, \min(b_2, b_3)))$$

By associativity of \min and \max , both sides are equal ✓

■

6. Absorption Laws

Theorem 6.1: $R_1 \mid (R_1 \& R_2) = R_1$

Proof: Case 1: $R_1 = \emptyset$

$$\emptyset \mid (\emptyset \& R_2) = \emptyset \mid \emptyset = \emptyset \quad \checkmark$$

Case 2: $R_2 = \emptyset$

$$R_1 \mid (R_1 \& \emptyset) = R_1 \mid \emptyset = R_1 \quad \checkmark$$

Case 3: Both $R_1 \neq \emptyset$ and $R_2 \neq \emptyset$

$$R_1 \& R_2 = (\max(l_1, l_2), \max(t_1, t_2), \min(r_1, r_2), \min(b_1, b_2))$$

If $R_1 \& R_2 = \emptyset$ (non-intersecting), then $R_1 \mid (R_1 \& R_2) = R_1 \mid \emptyset = R_1 \quad \checkmark$

If $R_1 \& R_2 \neq \emptyset$, then:

$$R_1 \mid (R_1 \& R_2) = (\min(l_1, \max(l_1, l_2)), \\ \min(t_1, \max(t_1, t_2)), \\ \max(r_1, \min(r_1, r_2)), \\ \max(b_1, \min(b_1, b_2)))$$

Since $l_1 \leq \max(l_1, l_2)$: $\min(l_1, \max(l_1, l_2)) = l_1$ Since $t_1 \leq \max(t_1, t_2)$: $\min(t_1, \max(t_1, t_2)) = t_1$ Since $r_1 \geq \min(r_1, r_2)$: $\max(r_1, \min(r_1, r_2)) = r_1$ Since $b_1 \geq \min(b_1, b_2)$: $\max(b_1, \min(b_1, b_2)) = b_1$

Therefore: $R_1 \mid (R_1 \& R_2) = (l_1, t_1, r_1, b_1) = R_1 \quad \checkmark$

■

Theorem 6.2: $R_1 \& (R_1 \mid R_2) = R_1$

Proof: Case 1: $R_1 = \emptyset$

$$\emptyset \& (\emptyset \mid R_2) = \emptyset \& R_2 = \emptyset \quad \checkmark$$

Case 2: $R_2 = \emptyset$

$$R_1 \& (R_1 \mid \emptyset) = R_1 \& R_1 = R_1 \quad \checkmark$$

Case 3: Both $R_1 \neq \emptyset$ and $R_2 \neq \emptyset$

$$R_1 \mid R_2 = (\min(l_1, l_2), \min(t_1, t_2), \max(r_1, r_2), \max(b_1, b_2))$$

$$R_1 \& (R_1 \mid R_2) = (\max(l_1, \min(l_1, l_2)), \\ \max(t_1, \min(t_1, t_2)), \\ \min(r_1, \max(r_1, r_2)), \\ \min(b_1, \max(b_1, b_2)))$$

Since $l_1 \geq \min(l_1, l_2)$: $\max(l_1, \min(l_1, l_2)) = l_1$ Since $t_1 \geq \min(t_1, t_2)$: $\max(t_1, \min(t_1, t_2)) = t_1$ Since $r_1 \leq \max(r_1, r_2)$: $\min(r_1, \max(r_1, r_2)) = r_1$ Since $b_1 \leq \max(b_1, b_2)$: $\min(b_1, \max(b_1, b_2)) = b_1$

Therefore: $R_1 \& (R_1 \mid R_2) = (l_1, t_1, r_1, b_1) = R_1 \checkmark$

■

7. Partial Order Properties

Theorem 7.1: Least Element ($\sqsubseteq \leq R_1$)

Proof: We must show $\sqsubseteq \& R_1 = \sqsubseteq$ for all R_1 .

By definition of meet: $\sqsubseteq \& R_1 = \sqsubseteq \checkmark$

Therefore $\sqsubseteq \leq R_1$ for all $R_1 \checkmark$

■

Theorem 7.2: Greatest Element ($R_1 \leq \sqsupseteq$)

Proof: We must show $R_1 \& \sqsupseteq = R_1$ for all R_1 .

This was proven in Theorem 1.2 \checkmark

Therefore $R_1 \leq \sqsupseteq$ for all $R_1 \checkmark$

■

Theorem 7.3: Reflexivity ($R_1 \leq R_1$)

Proof: We must show $R_1 \& R_1 = R_1$.

This was proven in Theorem 3.2 (idempotency of meet) \checkmark

■

Theorem 7.4: Transitivity ($R_1 \leq R_2 \wedge R_2 \leq R_3 \implies R_1 \leq R_3$)

Proof: Assume $R_1 \leq R_2$ and $R_2 \leq R_3$.

By definition: $R_1 \& R_2 = R_1$ and $R_2 \& R_3 = R_2$.

We must show $R_1 \& R_3 = R_1$.

$$\begin{aligned}
R_1 \& R_3 &= (R_1 \& R_2) \& R_3 && [\text{since } R_1 \& R_2 = R_1] \\
&= R_1 \& (R_2 \& R_3) && [\text{by associativity, Theorem 5.2}] \\
&= R_1 \& R_2 && [\text{since } R_2 \& R_3 = R_2] \\
&= R_1 && [\text{by assumption}]
\end{aligned}$$

Therefore $R_1 \leq R_3$ ✓

■

Theorem 7.5: Antisymmetry ($R_1 \leq R_2 \wedge R_2 \leq R_1 \implies R_1 = R_2$)

Proof: Assume $R_1 \leq R_2$ and $R_2 \leq R_1$.

By definition: $R_1 \& R_2 = R_1$ and $R_2 \& R_1 = R_2$.

By commutativity (Theorem 4.2): $R_1 \& R_2 = R_2 \& R_1$.

Therefore: $R_1 = R_1 \& R_2 = R_2 \& R_1 = R_2$ ✓

■

8. Monotonicity

Theorem 8.1: Join Monotonicity

Statement: If $R_1 \leq R_2$ and $R_3 \leq R_4$, then $R_1 \mid R_3 \leq R_2 \mid R_4$.

Proof: Assume $R_1 \leq R_2$ and $R_3 \leq R_4$.

By definition: $R_1 \& R_2 = R_1$ and $R_3 \& R_4 = R_3$.

For non-empty rectangles:

- If $R_1 = (l_1, t_1, r_1, b_1)$ and $R_2 = (l_2, t_2, r_2, b_2)$ with $R_1 \leq R_2$, then coordinate-wise: $l_2 \leq l_1 \leq r_1 \leq r_2$ and $t_2 \leq t_1 \leq b_1 \leq b_2$
- If $R_3 = (l_3, t_3, r_3, b_3)$ and $R_4 = (l_4, t_4, r_4, b_4)$ with $R_3 \leq R_4$, then coordinate-wise: $l_4 \leq l_3 \leq r_3 \leq r_4$ and $t_4 \leq t_3 \leq b_3 \leq b_4$

Then:

$$\begin{aligned}
R_1 \mid R_3 &= (\min(l_1, l_3), \min(t_1, t_3), \max(r_1, r_3), \max(b_1, b_3)) \\
R_2 \mid R_4 &= (\min(l_2, l_4), \min(t_2, t_4), \max(r_2, r_4), \max(b_2, b_4))
\end{aligned}$$

Since the inequalities hold coordinate-wise and \min/\max preserve order:

$$\min(l_2, l_4) \leq \min(l_1, l_3), \min(t_2, t_4) \leq \min(t_1, t_3)$$

$$\max(r_1, r_3) \leq \max(r_2, r_4), \max(b_1, b_3) \leq \max(b_2, b_4)$$

Therefore $R_1 \mid R_3 \leq R_2 \mid R_4$ ✓

■

Theorem 8.2: Meet Monotonicity

Statement: If $R_1 \leq R_2$ and $R_3 \leq R_4$, then $R_1 \& R_3 \leq R_2 \& R_4$.

Proof: Similar coordinate-wise argument as Theorem 8.1.

For non-empty rectangles with $R_1 \leq R_2$ and $R_3 \leq R_4$:

$$R_1 \& R_3 = (\max(l_1, l_3), \max(t_1, t_3), \min(r_1, r_3), \min(b_1, b_3))$$

$$R_2 \& R_4 = (\max(l_2, l_4), \max(t_2, t_4), \min(r_2, r_4), \min(b_2, b_4))$$

Since \min/\max preserve the coordinate inequalities:

$$\max(l_2, l_4) \leq \max(l_1, l_3), \max(t_2, t_4) \leq \max(t_1, t_3)$$

$$\min(r_1, r_3) \leq \min(r_2, r_4), \min(b_1, b_3) \leq \min(b_2, b_4)$$

Therefore $R_1 \& R_3 \leq R_2 \& R_4$ ✓

■

9. Completeness

Theorem 9.1: Arbitrary Joins Exist

Statement: For any $S \subseteq \text{Rect}$, the supremum $\bigvee S$ exists.

Proof: If $S = \emptyset$, define $\bigvee S = \sqempty$.

Otherwise, define:

$$L = \inf \{ l \mid (l, t, r, b) \in S, (l, t, r, b) \neq \sqempty \}$$

$$T = \inf \{ t \mid (l, t, r, b) \in S, (l, t, r, b) \neq \sqempty \}$$

$$R = \sup \{ r \mid (l, t, r, b) \in S, (l, t, r, b) \neq \sqempty \}$$

$$B = \sup \{ b \mid (l, t, r, b) \in S, (l, t, r, b) \neq \sqempty \}$$

and set:

$$\bigvee S = (L, T, R, B)$$

This rectangle is well-defined since $(L \leq R)$ and $(T \leq B)$.

For all $(R_i \in S)$, we have $(R_i \leq \bigvee S)$ by construction.

If (u) is any upper bound of (S) , then coordinate-wise:

$$l_u \leq L, t_u \leq T, R \leq r_u, B \leq b_u$$

hence $(\bigvee S \leq u)$.

Therefore $(\bigvee S)$ is the least upper bound of (S) ✓

■

Theorem 9.2: Arbitrary Meets Exist

Statement: For any $(S \subseteq \text{Rect})$, the infimum $(\bigwedge S)$ exists.

Proof: If $(S = \emptyset)$, define $(\bigwedge S = \boxed{})$.

Otherwise define:

$$\begin{aligned} L &= \sup \{ l \mid (l, t, r, b) \in S \} \\ T &= \sup \{ t \mid (l, t, r, b) \in S \} \\ R &= \inf \{ r \mid (l, t, r, b) \in S \} \\ B &= \inf \{ b \mid (l, t, r, b) \in S \} \end{aligned}$$

If $(L > R)$ or $(T > B)$, define $(\bigwedge S = \boxed{})$; otherwise:

$$\bigwedge S = (L, T, R, B)$$

For all $(R_i \in S)$, we have $(\bigwedge S \leq R_i)$ by construction.

If (m) is any lower bound of (S) , then coordinate-wise:

$$l_m \geq L, t_m \geq T, r_m \leq R, b_m \leq B$$

hence $(m \leq \bigwedge S)$.

Therefore $(\bigwedge S)$ is the greatest lower bound of (S) ✓

■

Corollary 9.3: Rect is a Complete Lattice

Statement: $(\text{Rect}, |, \&, \boxed{}, \boxed{})$ is a complete lattice.

Proof: By Theorems 9.1 and 9.2, arbitrary joins and meets exist ✓

■

10. Semidistributivity

Lemma 10.1: Meet Projections

Statement: For all (R_1, R_2) : $(R_1 \& R_2) \leq R_1$ and $(R_1 \& R_2) \leq R_2$.

Proof:

$$(R_1 \& R_2) \& R_1 = R_1 \& R_2 \quad [\text{by associativity and idempotency}]$$

$$(R_1 \& R_2) \& R_2 = R_1 \& R_2 \quad [\text{by associativity and idempotency}]$$

Therefore $(R_1 \& R_2) \leq R_1$ and $(R_1 \& R_2) \leq R_2$ ✓

■

Lemma 10.2: Join Injections

Statement: For all (R_1, R_2) : $R_1 \leq R_1 \mid R_2$ and $R_2 \leq R_1 \mid R_2$.

Proof:

$$R_1 \& (R_1 \mid R_2) = R_1 \quad [\text{by absorption, Theorem 6.2}]$$

$$R_2 \& (R_1 \mid R_2) = R_2 \quad [\text{by absorption, Theorem 6.2}]$$

Therefore $R_1 \leq R_1 \mid R_2$ and $R_2 \leq R_1 \mid R_2$ ✓

■

Theorem 10.3: Meet-Semidistributivity

Statement: $((R_1 \& R_2) \mid (R_1 \& R_3)) \leq R_1 \& (R_2 \mid R_3)$ for all (R_1, R_2, R_3) .

Proof: By Lemma 10.1:

$$(R_1 \& R_2) \leq R_1, \quad (R_1 \& R_3) \leq R_1$$

hence by monotonicity (Theorem 8.1):

$$(R_1 \& R_2) \mid (R_1 \& R_3) \leq R_1$$

Also by Lemma 10.1:

$$(R_1 \& R_2) \leq R_2, \quad (R_1 \& R_3) \leq R_3$$

hence by monotonicity:

$$(R_1 \& R_2) \mid (R_1 \& R_3) \leq R_2 \mid R_3$$

Since $(R_1 \& R_2) \mid (R_1 \& R_3) \leq R_1$ and $(R_1 \& R_2) \mid (R_1 \& R_3) \leq R_2 \mid R_3$:

$$(R_1 \& R_2) \mid (R_1 \& R_3) \leq R_1 \& (R_2 \mid R_3)$$

■

Theorem 10.4: Join-Semidistributivity

Statement: $R_1 \mid (R_2 \& R_3) \leq (R_1 \mid R_2) \& (R_1 \mid R_3)$ for all R_1, R_2, R_3 .

Proof: By Lemma 10.2:

$$R_1 \leq R_1 \mid R_2, \quad R_1 \leq R_1 \mid R_3$$

hence by monotonicity (Theorem 8.2):

$$R_1 \leq (R_1 \mid R_2) \& (R_1 \mid R_3)$$

Also by Lemma 10.1:

$$R_2 \& R_3 \leq R_2, \quad R_2 \& R_3 \leq R_3$$

hence by monotonicity:

$$R_2 \& R_3 \leq R_1 \mid R_2 \quad \text{and} \quad R_2 \& R_3 \leq R_1 \mid R_3$$

Therefore:

$$R_2 \& R_3 \leq (R_1 \mid R_2) \& (R_1 \mid R_3)$$

Since $R_1 \leq (R_1 \mid R_2) \& (R_1 \mid R_3)$ and $R_2 \& R_3 \leq (R_1 \mid R_2) \& (R_1 \mid R_3)$:

$$R_1 \mid (R_2 \& R_3) \leq (R_1 \mid R_2) \& (R_1 \mid R_3)$$

11. Failure of Modularity

The modular law states:

■ If $R_1 \leq R_2$, then $R_1 \mid (R_3 \ \& \ R_2) = (R_1 \mid R_3) \ \& \ R_2$

We demonstrate with an explicit counterexample that the Rect lattice is not modular.

Theorem 11.1: The Rect Lattice is Not Modular

Counterexample: Let:

$R_1 = (0, 0, 1, 1)$ [small 1×1 square]
 $R_2 = (0, 0, 1, 2)$ [1×2 rectangle containing R_1]
 $R_3 = (2, 0, 3, 2)$ [disjoint 1×2 rectangle]

Verify the precondition $R_1 \leq R_2$:

$R_1 \ \& \ R_2 = (\max(0, 0), \max(0, 0), \min(1, 1), \min(1, 2))$
 $= (0, 0, 1, 1)$
 $= R_1 \ \checkmark$

So indeed $R_1 \leq R_2$.

Left-hand side: $R_1 \mid (R_3 \ \& \ R_2)$

$R_3 \ \& \ R_2 = (\max(2, 0), \max(0, 0), \min(3, 1), \min(2, 2))$
 $= (2, 0, 1, 2)$
 $= \varnothing$ [since $2 > 1$]

$R_1 \mid (R_3 \ \& \ R_2) = R_1 \mid \varnothing$
 $= (0, 0, 1, 1)$
 $= R_1$

Right-hand side: $(R_1 \mid R_3) \ \& \ R_2$

$$R_1 \mid R_3 = (\min(0, 2), \min(0, 0), \max(1, 3), \max(1, 2)) \\ = (0, 0, 3, 2)$$

$$(R_1 \mid R_3) \& R_2 = (\max(0, 0), \max(0, 0), \min(3, 1), \min(2, 2)) \\ = (0, 0, 1, 2) \\ = R_2$$

Result:

$$R_1 \mid (R_3 \& R_2) = (0, 0, 1, 1) \neq (0, 0, 1, 2) = (R_1 \mid R_3) \& R_2$$

Therefore the modular law fails ✗

Geometric Intuition

The failure occurs because:

1. R_3 and R_2 are disjoint, so $R_3 \& R_2 = \emptyset$
2. The join $R_1 \mid R_3$ creates a **bounding box** that spans from R_1 to R_3 , including the empty space between them: $(0, 0, 3, 2)$
3. When this bounding box is intersected with R_2 , we get all of R_2 : $(0, 0, 1, 2)$
4. But the left side just gives us R_1 : $(0, 0, 1, 1)$

The key insight: **The join operation adds "virtual" space between disjoint rectangles.** This space persists through subsequent meet operations, violating the modular law's expectation that operations should be "well-behaved" when $R_1 \leq R_2$.

In a true modular lattice, the constraint $R_1 \leq R_2$ ensures that operations involving R_1 , R_2 , and any R_3 maintain certain symmetries. But in the Rect lattice, the bounding box operation breaks this symmetry by including regions that aren't actually part of either input rectangle.

■

12. Failure of Full Distributivity

Since distributivity implies modularity, and we have shown that modularity fails (Theorem 11.1), it follows that **distributivity must also fail**.

However, we provide an explicit counterexample to illustrate the specific manner in which distributivity fails in the Rect lattice.

Counterexample for $R_1 \& (R_2 \mid R_3) = (R_1 \& R_2) \mid (R_1 \& R_3)$

Consider:

$$R_1 = (0, 0, 4, 4)$$

$$R_2 = (1, 1, 7, 3)$$

$$R_3 = (5, 2, 6, 5)$$

Left side:

$$R_2 \mid R_3 = (1, 1, 7, 5)$$

$$\begin{aligned} R_1 \& (R_2 \mid R_3) &= (0, 0, 4, 4) \& (1, 1, 7, 5) \\ &= (\max(0, 1), \max(0, 1), \min(4, 7), \min(4, 5)) \\ &= (1, 1, 4, 4) \end{aligned}$$

Right side:

$$\begin{aligned} R_1 \& R_2 &= (0, 0, 4, 4) \& (1, 1, 7, 3) \\ &= (\max(0, 1), \max(0, 1), \min(4, 7), \min(4, 3)) \\ &= (1, 1, 4, 3) \end{aligned}$$

$$\begin{aligned} R_1 \& R_3 &= (0, 0, 4, 4) \& (5, 2, 6, 5) \\ &= (\max(0, 5), \max(0, 2), \min(4, 6), \min(4, 5)) \\ &= (5, 2, 4, 4) \\ &= \varnothing \text{ [since } 5 > 4\text{]} \end{aligned}$$

$$\begin{aligned} (R_1 \& R_2) \mid (R_1 \& R_3) &= (1, 1, 4, 3) \mid \varnothing \\ &= (1, 1, 4, 3) \end{aligned}$$

Result:

$$R_1 \& (R_2 \mid R_3) = (1, 1, 4, 4) \neq (1, 1, 4, 3) = (R_1 \& R_2) \mid (R_1 \& R_3)$$

Therefore distributivity fails ✗

Why This Happens Geometrically

The key insight is:

- $R_2 \mid R_3$ is the **bounding box** of R_2 and R_3 , which includes regions not in either R_2 or R_3
- When we intersect R_1 with this bounding box, we can include parts of R_1 that don't intersect either R_2 or R_3
- But $(R_1 \& R_2) \mid (R_1 \& R_3)$ only includes the parts of R_1 that actually intersect R_2 or R_3

In the example above:

- Rectangle R_3 doesn't intersect R_1 at all ($R_1 \& R_3 = \emptyset$)
- But $R_2 \mid R_3$ creates a bounding box that covers more area than just R_2 and R_3
- The bottom coordinate: $R_1 \& (R_2 \mid R_3)$ extends to 4 (from R_1), while $R_1 \& R_2$ only extends to 3 (from R_2)
- Since $R_1 \& R_3 = \emptyset$, the join $(R_1 \& R_2) \mid (R_1 \& R_3)$ is just $R_1 \& R_2 = (1, 1, 4, 3)$

■

Conclusion

We have proven that $(\text{Rect}, \mid, \&, \emptyset, \square)$ forms a **complete semidistributive lattice** with the following properties:

Proven to hold:

- ✓ Identity elements (\emptyset and \square)
- ✓ Absorbing elements
- ✓ Idempotency
- ✓ Commutativity
- ✓ Associativity
- ✓ Absorption laws
- ✓ Partial order properties (reflexivity, transitivity, antisymmetry, least and greatest elements)
- ✓ Monotonicity
- ✓ Completeness (arbitrary joins and meets exist)
- ✓ Semidistributivity (both inequalities)

Proven to fail:

- ✗ Full distributivity (equality fails in both laws)
- ✗ Modularity (fails even when precondition holds)

The precise classification is: **Complete Semidistributive Non-Modular Lattice**.